\author{Vincent Baguio}

\documentclass[letterpaper, 12pt]{article}
\usepackage[margin=1 in]{geometry}
\usepackage{amsmath,amssymb,amsfonts,amsthm,enumerate,cleveref,graphicx,fancyhdr}
\usepackage[framemethod=tikz]{mdframed}
\usepackage{subfiles}

\newmdenv{chest}{}
\pagestyle{empty}
\fancyhf{}

\rfoot{Page \thepage}
\lhead{\scriptsize 2020-01-14}
\rhead{\scriptsize MATH54}
\begin{document}
\thispagestyle{fancy}
\begin{Large}\textbf{Inverse Functions}\end{Large} \\

f(x) is the image of x under f while x is the pre-image f(x)\\

\textbf{One-to-one Function}: $f(x_{1}) \neq f(x_{2})$ whenever $x_{1} \neq x_{2}$

\textbf{Note: }Restrict the domain to make a non one-to-one function into a one-to-one function\\

\textbf{Cancellation Equations:}
\begin{align*}
f^{-1}((x)) &= x, \forall x \exists A\\
f(f^{-1}(x)) &= x, \forall x \exists B
\end{align*}

Quiz 1-16-2020

\textbf{Solutions:}\\
19. $h(x) = x + \sqrt{x}, h^{-1}(6)$

\begin{align*}
x + \sqrt{x} &= 6\\
\sqrt{x} &=  6 - x\\
x &= 36 - 12x + x^{2}\\
0 &= 36 - 13x + x^{2}\\
0 &= (9-x)(4-x)\\
x = 4, x = 9
\end{align*}

if x = 4
\begin{align*}
h(4) &=  4 + \sqrt{4}\\ 
&=  4 + 2 = 6
\end{align*}

if x = 9
\begin{align*}
h(9) &=  9 + \sqrt{9}\\
&= 9 + 3 = 12
\end{align*}
Therefore x = 4 and $h^{-1}(6) = 4$\\

27. $y = \frac{1-\sqrt{x}}{1+\sqrt{x}}$
\begin{align*}
y + y\sqrt{x} &= 1 - \sqrt{x}\\
\sqrt{x} + y \sqrt{x} &= 1-y\\
\sqrt{x}(1+y)&= 1-y\\
\sqrt{x} &= \frac{1-y}{1+y}\\
x &= \left(\frac{1-y}{1+y}\right) ^{2}\\
y &= \left(\frac{1-x}{1+x}\right) ^{2}\\
f^{-1}(x) &= \left(\frac{1-x}{1+x}\right) ^{2}
\end{align*}

40. $f(x)= 2x^{3} + 3x^{2} + 7x + 4, a = 4$\\
$f'(x) = 6x^{2}	+ 6x + 7$\\
\begin{align*}
	(f^(-1))'(4) &= \frac{1}{f'(f^(-1)(4))}\\
	2x^{3} + 3x^{2}	+7x + 4 &=  4\\
	2x^{3} +3x^{2}	+7x &=  0\\
	x(2x^{2} + 3x + 7) &= 0\\
\end{align*}

Therefore x = 4 and $f^{-1}(4) = 0$

\begin{align*}
&= \frac{1}{f^{-1}(0)}\\
&= \frac{1}{6(0)^{2}+6(0)+7}\\
&= (f^{-1})'(4)=\frac{1}{7}
\end{align*}
\end{document}
